proof for replacing empty in a context

Hs/Metatheory/Substitution.lean
@@ -3,6 +3,7 @@ import Hs.HsJudgment
 import SystemFD.Ctx
 import Hs.Metatheory.TypeMatch
 import Hs.Metatheory.Weaken
+import Hs.Metatheory.FrameWf
 
 set_option maxHeartbeats 1000000
 
@@ -431,22 +432,150 @@ case _ =>
   simp at h1
 
 
-def hs_replace_empty : (v : HsVariant) ->  {idx : HsJudgmentArgs v} ->
-  HsJudgment v (.empty :: Γ) idx ->
-  Γ ⊢τ A : `★ ->
-  HsJudgment v (.type A :: Γ) idx
-| .ctx, () , j, j' => by
-  cases j; constructor; assumption; assumption
-| .kind, (t, τ), j, j' => match j with
-  | .ax h => by apply HsJudgment.ax; cases h; case _ h => apply HsJudgment.wftype; assumption; assumption
-  | .arrowk h1 h2 => by apply HsJudgment.arrowk (hs_replace_empty .kind h1 j') (hs_replace_empty .kind h2 j')
-| .type, (t, τ), j, j' => sorry
-| .term, (t, τ), j, j' => sorry
-termination_by _ _ h => h.size
+def hs_replace_empty_kind : (k : HsTerm) ->
+  (.empty :: Γ) ⊢κ k : s ->
+  Γ ⊢s f ->
+  (f :: Γ) ⊢κ k : s := by
+intro k j1 j2
+have wf := hs_judgment_ctx_wf .kind j1
+cases wf; case _ wf =>
+have lem := Ctx.weaken_frame wf j2
+cases j1
+case _ h => constructor; assumption
+case _ k1 k2 h1 h2 =>
+  have h1' := hs_replace_empty_kind k1 h1 j2
+  have h2' := hs_replace_empty_kind k2 h2 j2
+  constructor; assumption; assumption
+termination_by h => h.size -- this is hilariously stupid lean4
 
+
+theorem empty_never_indexed_kind : (t A : HsTerm) ->
+  (Γ d@ n) = .empty ->
+  Γ ⊢κ t : A ->
+  n ∉ t.fvs ∧ n ∉ A.fvs := by
+intro _ _ h1 h2;
+cases h2;
+case _ => simp
+case _ A B ih1 ih2 =>
+have lem1 := empty_never_indexed_kind A `□ h1 ih1
+have lem2 := empty_never_indexed_kind B `□ h1 ih2
+cases lem1; cases lem2
+simp; constructor; assumption; assumption
+termination_by h => h.size
+
+theorem empty_never_indexed_type : (t A : HsTerm) ->
+  (Γ d@ n) = .empty ->
+  Γ ⊢τ t : A ->
+  n ∉ t.fvs ∧ n ∉ A.fvs := by sorry
+
+
+theorem empty_never_indexed_term : (t A : HsTerm) ->
+  (Γ d@ n) = .empty ->
+  Γ ⊢t t : A ->
+  n ∉ t.fvs ∧ n ∉ A.fvs := by sorry
+
+
+def hs_replace_kind_lemma : (τ k : HsTerm) -> (Γ Γ' : Ctx HsTerm) ->
+  (Γ d@ n) = .empty ->
+  Γ.drop (n + 1) ⊢s f ->
+  Γ.modify n (λ _ => f) = Γ' ->
+  Γ ⊢κ τ : k ->
+  Γ' ⊢κ τ : k := by sorry
+
+
+theorem n_x_different : (Γ : Ctx HsTerm) ->
+  Γ d@ n = .empty ->
+  (Γ d@ x).get_type = .some k ->
+  x ≠ n := by
+intro Γ j1 j2 j3;
+rw[j3] at j2; rw[j1] at j2; unfold Frame.get_type at j2; simp at j2;
+
+def hs_replace_type_lemma : (τ k : HsTerm) -> (Γ Γ' : Ctx HsTerm) ->
+  (Γ d@ n) = .empty ->
+  Γ.drop (n + 1) ⊢s f ->
+  Γ.modify n (λ _ => f) = Γ' ->
+  ⊢s Γ' ->
+  Γ ⊢τ τ : k ->
+  Γ' ⊢τ τ : k := by
+intro τ k Γ Γ' j1 j2 j3 j4 j5;
+have lem : ∀ f, (f :: Γ) d@ (n + 1) = .empty := by intro f; simp; unfold Frame.apply; rw[j1]
+cases j5;
+case _ A B h1 h2 =>
+  constructor;
+  apply hs_replace_kind_lemma A `□ Γ Γ' j1 j2 j3 h1
+  apply hs_replace_type_lemma B `★ (.kind A :: Γ) (.kind A :: Γ');
+  apply lem
+  assumption
+  simp; assumption
+  constructor;
+  apply hs_replace_kind_lemma A `□ Γ Γ' j1 j2 j3 h1
+  assumption
+  assumption
+case _ A B h1 h2 =>
+  constructor
+  apply hs_replace_type_lemma A `★ Γ Γ' j1 j2 j3 j4 h1
+  apply hs_replace_type_lemma B `★ (.empty :: Γ) (.empty :: Γ');
+  apply lem
+  assumption
+  simp; assumption
+  constructor; assumption
+  assumption
+case _ A B h1 h2 h3 =>
+  constructor
+  apply hs_replace_type_lemma A `★ Γ Γ' j1 j2 j3 j4 h1
+  apply hs_replace_empty_valid_head_variable_opent Γ Γ' j1 j3 h2
+  apply hs_replace_type_lemma B `★ (.empty :: Γ) (.empty :: Γ');
+  apply lem
+  assumption
+  simp; assumption
+  constructor; assumption
+  assumption
+case _ f A a h1 h2 h3 h4 =>
+  constructor;
+  apply hs_replace_type_lemma f (A `-k> k) Γ Γ' j1 j2 j3 j4 h3
+  apply hs_replace_type_lemma a A Γ Γ' j1 j2 j3 j4 h1
+  apply hs_replace_kind_lemma A `□ Γ Γ' j1 j2 j3 h2
+  apply hs_replace_kind_lemma k `□ Γ Γ' j1 j2 j3 h4
+case _ x wf h1 h2 h3 =>
+  have lem1 := n_x_different Γ j1 (Eq.symm h2)
+  have lem2 := replace_eq_except Γ Γ' j3 x lem1
+  constructor;
+  assumption
+  case _ => rw [<-lem2]; assumption
+  case _ => rw [<-lem2]; assumption
+  apply hs_replace_kind_lemma k `□ Γ Γ' j1 j2 j3 h3
+
+termination_by h => h.size
+
+#eval ([1,2,3]).modify 1 (λ _ => 5)
+#eval ([1,2,3].take 1 ++ [5] ++ [1,2,3].drop 2)
+
+
+def hs_replace_empty_type_lemma : (τ : HsTerm) ->
+  (.empty :: Γ) ⊢τ τ : k ->
+  Γ ⊢s f ->
+  (f :: Γ) ⊢τ τ : k := by
+intro τ j f;
+have lem1 : (.empty :: Γ) d@ 0 = .empty := by simp; unfold Frame.apply; simp
+apply hs_replace_type_lemma
+assumption
+assumption
+unfold List.modify; simp
+apply Ctx.weaken_frame; apply hs_frame_wf_implies_wf f; assumption
+assumption
 
 def hs_replace_empty_type :
   Γ ⊢τ A : `★ ->
   (.empty :: Γ) ⊢τ B : `★ ->
-  (.type A :: Γ) ⊢τ B : `★
-:= λ a b => hs_replace_empty .type b a
+  (.type A :: Γ) ⊢τ B : `★ :=
+by
+intro j1 j2
+have wf := hs_judgment_ctx_wf .type j1
+have lem : Γ ⊢s (.type A) := by constructor; assumption
+apply hs_replace_empty_type_lemma; assumption; assumption
+
+
+def hs_replace_term : (t : HsTerm) ->
+  (.empty :: Γ) ⊢t t : τ ->
+  Γ ⊢s f ->
+  (f :: Γ) ⊢t t : τ := by sorry
