Hs/Metatheory/SubstitutionCompile.lean
@@ -7,6 +7,7 @@ import Hs.Metatheory.WeakenCompile
 import Hs.Metatheory.Substitution
 import Hs.Algorithm
 
+
 theorem compile_beta_kind_type :
   (j1 : (.kind A::Γ) ⊢τ b : B) ->
   compile_type (.kind A::Γ) b B j1 = .some b' ->
@@ -31,3 +32,9 @@ theorem compile_beta_empty_term :
   compile_term Γ t A j2 = .some t' ->
   (j3 : Γ ⊢τ (b β[t]) : (B β[t])) ->
   compile_type Γ (b β[t]) (B β[t]) j3 = .some (b' β[t']) := by sorry
+
+def compile_replace_empty :
+  (j1 : (.empty :: Γ) ⊢τ τ : k) ->
+  (j2 : (f :: Γ) ⊢τ τ : k) ->
+  compile_type (.empty :: Γ) τ k j1 = .some τ' ->
+  compile_type (f :: Γ) τ k j2 = .some τ' := by sorry
